src/Lean/Environment.lean
@@ -735,7 +735,7 @@ private def setImportedEntries (env : Environment) (mods : Array ModuleData) (st
   let extDescrs ← persistentEnvExtensionsRef.get
   /- For extensions starting at `startingAt`, ensure their `importedEntries` array have size `mods.size`. -/
   for extDescr in extDescrs[startingAt:] do
-    env := extDescr.toEnvExtension.modifyState env fun s => { s with importedEntries := mkArray mods.size #[] }
+    env := extDescr.toEnvExtension.modifyState env fun s => { s with importedEntries := Array.replicate mods.size #[] }
   /- For each module `mod`, and `mod.entries`, if the extension name is one of the extensions after `startingAt`, set `entries` -/
   let extNameIdx ← mkExtNameMap startingAt
   for h : modIdx in [:mods.size] do
